checks/SemantChecks.v
@@ -5,13 +5,32 @@ Require Import Semant.
 Require Import Types.
 
 Section TypeDec_CHECKS.
-
+  (* With soundness this also implies wt_prog ex ty us *)
   Definition checkEx (ex : Absyn.exp) :=
     exists ty us, transProg ex = OK (ty, us).
 
-  Ltac solve := 
+  (* With soundness this implies that transProg ex = ERR *)
+  Definition failEx (ex : Absyn.exp) := forall ty us,
+    ~(wt_prog ex ty us).
+
+  Ltac inv H := inversion H; subst; clear H.
+  Ltac inv_all :=
+    repeat match goal with
+    | [ H : wt_prog _ _ _ |- _ ] => inv H
+    | [ H : wt_exp _ _ _ _ _ |- _ ] => inv H
+    | [ H : wt_op _ _ _ _ |- _ ] => inv H
+    | [ H : Some _ = Some _ |- _ ] => inv H
+    | [ H : Some _ = None |- _ ] => inv H
+    | [ H : None = Some _ |- _ ] => inv H
+    | [ H : None = None |- _ ] => inv H
+    | [ H : Types.actual_ty _ Types.STRING = Some _ |- _] => unfold Types.actual_ty in H; simpl in H
+    | [ H : Types.actual_ty _ Types.INT = Some _ |- _] => unfold Types.actual_ty in H; simpl in H
+    end; simpl in *; try discriminate.
+
+  Ltac solve :=
     match goal with
-    | [ |- checkEx ?E ] => unfold checkEx; unfold E; unfold transProg; simpl; eauto
+    | [ |- checkEx ?E ] => unfold checkEx, E, transProg; simpl; eauto
+    | [ |- failEx ?E ] => unfold failEx, E, not; intros; inv_all
     end.
 
   Example ex1 : checkEx EX1.ex.
@@ -21,6 +40,30 @@ Section TypeDec_CHECKS.
   Proof. solve. Qed.
 
   Example ex3 : checkEx EX3.ex.
+  Proof. solve. Qed.
+
+  Example ex4 : checkEx EX4.ex.
+  Proof. solve. Qed.
+
+  Example ex5 : checkEx EX5.ex.
+  Proof. solve. Qed.
+
+  Example ex6 : checkEx EX6.ex.
+  Proof. solve. Qed.
+
+  Example ex7 : checkEx EX7.ex.
+  Proof. solve. Qed.
+
+  Example ex8 : checkEx EX8.ex.
+  Proof. solve. Qed.
+
+  Example ex9 : failEx EX9.ex.
+  Proof. solve. Qed.
+
+  Example ex10 : failEx EX10.ex.
+  Proof. solve. Qed.
+
+  Example ex11 : failEx EX11.ex.
   Proof. solve. Qed.
 
 End TypeDec_CHECKS.
